rustfrontend/RustIRgenProof.v
@@ -16,12 +16,10 @@ Local Open Scope list_scope.
 Local Open Scope error_monad_scope.
 
 (** Semantics preservation of the generation of RustIR programs from
-Rustlight programs. The key parts of the proof are to 1. relate the
+Rustlight programs. The key part of the proof is to relate the
 semantics drops expressed in the continuation to the drop statements
-explicitly inserted in the program; 2. handle the discrepency between
-the source (mem, env, own_env) and the target (mem, env, own_env) due
-to the new generated return variable which is used to store the return
-value before dropping all the in-scope variables and parameters. *)
+explicitly inserted in the program *)
+
 
 Definition match_glob (ctx: composite_env) (gd: globdef Rustlight.fundef type) (tgd: globdef RustIR.fundef type) : Prop :=
   match gd, tgd with
@@ -45,7 +43,7 @@ Record match_prog (p : Rustlight.program) (tp : RustIR.program) : Prop := {
     generate_dropm p = RustIR.generate_dropm tp;
     match_prog_skel:
     erase_program tp = erase_program p;
-}.
+  }.
 
 
 Section PRESERVATION.
@@ -55,7 +53,6 @@ Variable prog: program.
 Variable tprog: RustIR.program.
 
 Hypothesis TRANSL: match_prog prog tprog.
-Variable w: inj_world.
 
 Variable se: Genv.symtbl.
 Variable tse: Genv.symtbl.
@@ -64,37 +61,126 @@ Variable tse: Genv.symtbl.
 Let ge := globalenv se prog.
 Let tge := RustIR.globalenv tse tprog.
 
+Inductive match_drop_insert_kind: drop_insert_kind -> RustIR.statement -> Prop :=
+| match_drop_reassign: forall p,
+    match_drop_insert_kind (drop_reassign p) (gen_drop ge p)
+| match_drop_escape: forall l,
+    match_drop_insert_kind (drop_escape l) (gen_drops_for_escape_vars ge l)
+| match_drop_return: forall l,
+    match_drop_insert_kind (drop_return l) (gen_drops_for_vars ge l)
+| match_drop_reassign_end:
+  match_drop_insert_kind drop_reassign_end RustIR.Sskip
+.
+
+
+(* We distinguish the dropcont from reassign purpose and out-of-scope
+purpose *)
+
+Inductive match_dropcont : dropcont -> RustIR.statement -> Prop :=
+| match_Dassign: forall p e,
+    match_dropcont (Dassign p e) (RustIR.Sassign p e)
+| match_Dassign_variant: forall p e eid fid,
+    match_dropcont (Dassign_variant p eid fid e) (RustIR.Sassign_variant p eid fid e)
+| match_Dbox: forall p e,
+    match_dropcont (Dbox p e) (RustIR.Sbox p e)
+| match_Dcall: forall p a al,
+    match_dropcont (Dcall p a al) (RustIR.Scall p a al)
+| match_Dbreak:
+  match_dropcont Dbreak RustIR.Sbreak
+| match_Dcontinue:
+  match_dropcont Dcontinue RustIR.Scontinue
+| match_Dendlet:
+  (* may be we should generate sskip in the end of the let *)
+  match_dropcont Dendlet RustIR.Sskip
+.
+
+
+Inductive match_cont (params: list (ident * type)) : cont -> RustIRown.cont -> Prop :=
+| match_Klet: forall k tk drop id ty
+    (MCONT: match_cont params k tk)
+    (DROP: drop = gen_drop ge (Plocal id ty)),
+    (* when executing Klet, Rustlight would enter Dropinsert state
+    where drop_escape contains the out-of-scope variable which is
+    related to (drop;storagedead id) *)
+    match_cont params (Klet id ty k) (RustIRown.Kseq (RustIR.Ssequence drop (Sstoragedead id)) tk)
+(* The drops are inserted for the reassignment. The translated
+statement does not contain storagedead *)
+| match_Kdropinsert: forall k tk dk s1 s2 st
+    (MCONT: match_cont params k tk)
+    (MDCONT: match_dropcont dk s2)
+    (MDINS: match_drop_insert_kind st s1),
+    match_cont params (Kdropinsert st dk k)
+      (RustIRown.Kseq (RustIR.Ssequence s1 s2) tk)
+| match_Kstop:
+    match_cont params Kstop RustIRown.Kstop
+| match_Kseq: forall k s tk ts
+    (TRSTMT: transl_stmt ge params s (cont_vars k) = ts)
+    (MCONT: match_cont params k tk),
+    match_cont params (Kseq s k) (RustIRown.Kseq ts tk)
+| match_Kloop: forall k tk s ts
+    (MCONT: match_cont params k tk)
+    (TRSTMT: transl_stmt ge params s (cont_vars k) = ts),
+    match_cont params (Kloop s k) (RustIRown.Kloop ts tk)
+| match_Kcall: forall k tk p f tf le own
+    (TRFUN: transl_function ge f = tf)
+    (MCONT: match_cont f.(fn_params) k tk),
+    match_cont params (Kcall p f le own k) (RustIRown.Kcall p tf le own tk)
+| match_Kdropplace: forall k tk f tf st drops le own
+    (MCONT: match_cont f.(fn_params) k tk)
+    (TRFUN: transl_function ge f = tf),
+    match_cont params (Kdropplace f st drops le own k) (RustIRown.Kdropplace tf st drops le own tk)
+| match_Kdropcall: forall k tk id v st membs
+    (MCONT: match_cont params k tk),
+    match_cont params (Kdropcall id v st membs k) (RustIRown.Kdropcall id v st membs tk)
+.
+     
 Inductive match_states: Rustlightown.state -> RustIRown.state -> Prop := 
-| match_regular_state: 
-  forall f s k e own m tf ts tk te town tm oretv vars j
-    (* It is no need to relate two functions *)
-    (TRSTMT: transl_stmt ge f.(fn_params) oretv s vars = ts)
+| match_regular_state: forall f s k e own m tf ts tk vars
+    (TRFUN: transl_function ge f = tf)
+    (TRSTMT: transl_stmt ge f.(fn_params) s vars = ts)
     (* The in-scope variables collected in transl_stmt are the same as
     those collected in the continuation *)
     (CONTVARS: cont_vars k = vars)
-    (* relation between (e, own) and (te, town) *)
-    (MENV: 
-    (MINJ: Mem.inject j m tm),
-    match_states (State f s k e own m) (RustIRown.State tf ts tk te town tm) 
-| match_dropinsert_state:
-  forall f l dk k le own m tf ts tk te town tm j
-    (MINJ: Mem.inject j m tm),
-    (* Dropinsert f l dk k le own m *)
-    match_states (Dropinsert f l dk k le own m) (RustIRown.State tf ts tk te town tm).
-
-
+    (MCONT: match_cont f.(fn_params) k tk),
+    match_states (State f s k e own m) (RustIRown.State tf ts tk e own m)
+| match_dropinsert: forall f tf st dk k tk le own m ts1 ts2
+    (TRFUN: transl_function ge f = tf)
+    (STMT1: match_drop_insert_kind st ts1)
+    (STMT2: match_dropcont dk ts2)
+    (MCONT: match_cont f.(fn_params) k tk),
+    match_states (Dropinsert f st dk k le own m) (RustIRown.State tf ts1 (RustIRown.Kseq ts2 tk) le own m)
+| match_dropplace: forall f tf k tk st drops le m own
+    (TRFUN: transl_function ge f = tf)
+    (MCONT: match_cont f.(fn_params) k tk),
+    match_states (Dropplace f st drops k le own m) (RustIRown.Dropplace tf st drops tk le own m)
+| match_dropstate: forall id v st membs k tk m
+    (* We does not care the parameters in drop glue state *)
+    (MCONT: forall l, match_cont l k tk),
+    match_states (Dropstate id v st membs k m) (RustIRown.Dropstate id v st membs tk m)
+| match_callstate: forall v al k tk m
+    (MCONT: forall l, match_cont l k tk),
+    match_states (Callstate v al k m) (RustIRown.Callstate v al tk m)
+| match_returnstate: forall v k tk m
+    (MCONT: forall l, match_cont l k tk),
+    match_states (Returnstate v k m) (RustIRown.Returnstate v tk m)
+.
 
 
 Lemma step_simulation:
   forall S1 t S2, step ge S1 t S2 ->
   forall S1' (MS: match_states S1 S1'), exists S2', plus RustIRown.step tge S1' t S2' /\ match_states S2 S2'.
 Proof.
-  induction 1; intros. 
-  - inv MS. simpl. destruct (own_type (prog_comp_env prog) (typeof_place p)) eqn:A. 
-    + eexists. split. eapply plus_one. eapply RustIRown.step_seq. 
-      econstructor. eauto. 
-    + eexists. split. eapply plus_one. econstructor; eauto.       
-      
+  induction 1; intros; inv MS.
+  - simpl.
+    eexists. split.
+    (* step *)
+    econstructor. econstructor.
+    eapply star_refl. auto.
+    econstructor; auto.
+    unfold gen_drop, gen_drops.
+    destruct (own_type (prog_comp_env prog) (typeof_place p)); auto.
+    econstructor.
+    
   Admitted. 
 
 (* Theorem transl_program_correct prog tprog:
